basic mac then encrypt example

examples/crypto/AES.fst
@@ -7,10 +7,13 @@ type bytes = Bytes.bytes // TODO unclear why we need this instead of seq byte
 type nbytes (n:nat) = b:bytes{Bytes.length b == n}
 
 let blocksize = 32 (* 256 bits *)
+let psize = blocksize
+let csize = (op_Multiply 2 blocksize)
 
-type plain  = nbytes blocksize
 
-type cipher = nbytes (op_Multiply 2 blocksize)  (* including IV *)
+type plain  = nbytes psize
+type cipher = nbytes csize  (* including IV *)
+
 
 let keysize = 16 (* 128 bits *)
 type key = nbytes keysize 
@@ -21,4 +24,4 @@ assume val generated : key -> Tot bool
 
 assume val gen: unit -> key 
 assume val dec: key -> cipher -> Tot plain                    (* this function is pure & complete *)  
-assume val enc: k:key -> p:plain -> c:cipher { dec k c = p }  (* this function is not pure (IV); the refinement captures functional correctness *) 
+assume val enc: k:key -> p:plain -> Tot (c:cipher { dec k c = p })  (* this function is not pure (IV); the refinement captures functional correctness *) 
