examples/crypto/MtE.CPA.fst
@@ -1,0 +1,70 @@
+module MtE.CPA
+
+open FStar.Heap
+(* open FStar.HyperHeap *)
+open FStar.Seq
+open FStar.SeqProperties
+(* open FStar.Monotonic.RRef *)
+
+open Platform.Bytes
+open CoreCrypto
+
+open MtE.Plain
+
+
+type cipher = AES.cipher
+
+
+
+type entry = // records that c is an encryption of p with ad
+  | Entry: p:plain -> c:cipher -> entry
+
+let ideal_log : ref (seq entry) = alloc (createEmpty #entry)
+
+
+abstract type key = AES.key
+
+assume type encrypted: key -> bytes -> Type
+
+let keysize = 16
+
+val keygen: unit -> key
+let keygen () =
+  AES.gen ()
+
+
+val encrypt: (k:key) -> (p:plain) -> ST (c:cipher{encrypted k c})
+  (requires (fun h -> true))
+  (ensures (fun h0 c h2 -> ind_cpa ==> (let log = (Heap.sel h2 ideal_log) in exists (i:nat{i < Seq.length log}).  Seq.index log i == Entry p c)) )
+
+ 
+let encrypt k p =
+  let text = if ind_cpa then createBytes AES.psize 0z else repr p in
+  let c = (AES.enc k text) in
+  if ind_cpa then
+    ideal_log := snoc !ideal_log (Entry p c);
+  assume(encrypted k c);
+  c
+  
+
+val decrypt: (k:key) -> (c:cipher) -> ST (p:plain)
+  (requires (fun h -> (let s = (Heap.sel h ideal_log) in is_Some (seq_find (function Entry c' p -> c=c') s))) )
+  (ensures (fun h0 c h2 -> true))
+
+//  (requires (fun h -> (let log = (Heap.sel h ideal_log) in exists (i:nat{i < Seq.length log}). exists (p:plain).  Seq.index log i = Entry c p) ))
+
+
+let decrypt (k:key) (c:cipher)=
+  if ind_cpa then 
+  begin
+    let s = !ideal_log in
+    match seq_find (function Entry c' p -> c=c') s with
+    | Some e -> (Entry.p e )
+  end
+  else
+    AES.dec k c
+
+let test =
+  let p = createBytes 1 0z in
+  let k = keygen () in
+  ignore (encrypt k (createBytes 32 0z))
