examples/crypto/MtE.Plain.fst
@@ -1,0 +1,15 @@
+module MtE.Plain
+
+open Platform.Bytes
+
+
+type plain = AES.plain
+
+val ind_cpa : bool
+let ind_cpa = false
+
+assume val repr: p:plain{ind_cpa == false} -> Tot (AES.plain)
+
+
+assume val mk_plain: r:bytes{ind_cpa == false} -> Tot (plain)
+
